theories/DecisionProcedure.v
@@ -93,44 +93,238 @@ Proof.
 intros. exists c;auto.
 Qed.
 
+Ltac d_ctx := unfold In_mod_R in *;destruct_ctx.
+
 Lemma In_mod_R_cons : forall c c' l, In_mod_R c l -> In_mod_R c (c' :: l).
 Proof.
-intros. unfold In_mod_R in *. destruct_ctx. exists x. split;auto.
+intros. d_ctx. exists x. split;auto.
 Qed.
 
 Hint Resolve In_mod_R_eq In_mod_R_cons : dpDB.
 
- 
 
+Lemma In_mod_R_app : forall l0 l1 c, In_mod_R c l0 \/ In_mod_R c l1 -> In_mod_R c (l0++l1).
+Proof.
+induction l0;intros. simpl. destruct H.
+d_ctx. simpl in H0. contradiction. auto.
+inversion H.
+- d_ctx. exists x. split;auto. apply in_or_app. now left.
+- d_ctx. exists x. split;auto. apply in_or_app. now right.
+Qed.
+
+Notation "l0 =L= l1" := (plus_fold l0 =R= plus_fold l1) (at level 73, no associativity).
+
+
+Definition In_mod_ACI (c : Contract) (l : list Contract) := exists c', c' =ACI= c /\ In c' l.
+
+Ltac dd_ctx := unfold In_mod_ACI in *;destruct_ctx.
 
 CoInductive AllDerivatives : Contract -> list Contract -> Prop :=
-| AD_fix c l (H0: forall e, AllDerivatives (c/e) l) (H1 : In c l)  : AllDerivatives c l
-| AD_sub c0 c1 l (H0: c0 =R= c1) (H1: AllDerivatives c0 l)  : AllDerivatives c1 l. (*Report: Necessary constructor for substitution because of Coq's guardedness constraint*)
+| AD_fix c l (H0: forall e, AllDerivatives (c/e) l) (H1 : In_mod_ACI c l)  : AllDerivatives c l.
+
+Definition is_FailureConf (ll : list (list Contract)) := ll<>[] /\  forall l, In l ll -> In Failure l.
+
+Print NoDup.
+
+Inductive In_mod_LACI : list Contract -> list (list Contract) -> Prop :=
+| Iml_nil : In_mod_LACI [] []
+| Iml_extend_ll l l' ll (H: In_mod_LACI l ll) : In_mod_LACI l (l'::ll)
+| Iml_extend_l c l ll (H0: exists l', In l' ll /\ In c l') (H1: In_mod_LACI l ll) : In_mod_LACI (c::l) ll.
+
+Equations n_prod_list (A:Type)(ll : list (list A)) : list (list A) by wf (length ll) lt :=
+n_prod_list [] := [[]];
+n_prod_list (l::ll') := map (fun p => (fst p)::(snd p)) (list_prod l (n_prod_list (ll'))).
+Global Transparent n_prod_list.
+
+Definition f_extend (ll : list (list Contract)) := map (fun l => l++[Failure]) ll.
+
+Lemma in_n_prod_list_extend : forall (l l' : list Contract) e(ll : list (list Contract)),
+ In l (n_prod_list ll) -> In e l' -> In (e::l) (n_prod_list (l'::ll)).
+Proof.
+induction l;intros.
+- simp n_prod_list. rewrite in_map_iff.
+  exists (e,[]). split;auto. apply in_prod;auto.
+- simp n_prod_list. rewrite in_map_iff.
+  exists (e,a::l). split;auto. apply in_prod;auto.
+Qed.
+
+Lemma in_n_prod_cons : forall (l l' : list Contract) e(ll : list (list Contract)),
+ In (e::l) (n_prod_list (l'::ll)) -> In e l' /\ In l (n_prod_list ll).
+Proof.
+intros. simp n_prod_list in H. rewrite in_map_iff in H.
+d_ctx. inversion H. subst. destruct x.
+rewrite in_prod_iff in H0. simpl.
+destruct H0;auto.
+Qed.
+
+Lemma in_n_prod_iff : forall (l l' : list Contract) e(ll : list (list Contract)),
+ In (e::l) (n_prod_list (l'::ll)) <-> In e l' /\ In l (n_prod_list ll) .
+Proof.
+split;intros. auto using in_n_prod_cons.
+destruct H. auto using in_n_prod_list_extend.
+Qed.
+
+Lemma in_n_prod_app : forall (l l' : list Contract) (ll ll' : list (list Contract)),
+ In l (n_prod_list ll) -> In l' (n_prod_list ll')  -> In (l++l') (n_prod_list (ll++ll')).
+Proof.
+induction l;intros;simpl.
+- destruct ll. simpl in H. destruct H;try contradiction.
+  auto. simp n_prod_list in H. rewrite in_map_iff in H.
+  d_ctx. discriminate.
+- destruct ll. simpl. simpl in H. destruct H;try contradiction. 
+  discriminate. rewrite <- app_comm_cons. rewrite in_n_prod_iff. 
+  rewrite in_n_prod_iff in H. destruct H;auto.
+Qed.
+
+Lemma in_n_prod_repeat : forall (A:Type) (n:nat) (e:A) (l:list A) ,
+ In e l-> In (repeat e n) (n_prod_list (repeat l n)).
+Proof.
+intro. induction n;intros;simpl. now left.
+apply IHn in H as H'. simp n_prod_list.
+ rewrite in_map_iff. exists (e,repeat e n).
+split;auto. rewrite in_prod_iff. split;auto.
+Qed.
+
+Lemma In_mod_LACI_f_extend : forall ll, In_mod_LACI [] (f_extend ll).
+Proof.
+induction ll;intros;simpl. constructor. constructor.
+auto.
+Qed.
+
+Lemma Failure_plus_fold : forall l, Failure _+_ (plus_fold l) =ACI= plus_fold l.
+Proof.
+induction l;intros;simpl;auto. rewrite cc_plus_comm.
+rewrite cc_plus_assoc.
+apply cc_ctx_plus;auto. rewrite cc_plus_comm. auto.
+Qed.
 
 
-(*
-Inductive OnlyDerivatives : Contract -> list Contract -> Prop :=
-| OD_nil c : OnlyDerivatives c [c]
-| OD_cons c c' l e (H: In_mod_R c' l) (H1: OnlyDerivatives c 
-*)
+Lemma In_plus_Failure : forall l ll, In_mod_ACI (plus_fold l) ll-> In_mod_ACI (Failure _+_ plus_fold l) ll.
+Proof.
+induction l;intros. 
+- simpl in *. dd_ctx. exists x. split. rewrite H. all: auto.
+- dd_ctx. exists x. split. simpl in H. rewrite H. rewrite Failure_plus_fold.
+  now simpl. auto.
+Qed. 
+
+Lemma In_plus_Failure2 : forall l ll, In_mod_ACI (Failure _+_ plus_fold l) ll -> In_mod_ACI (plus_fold l) ll.
+Proof.
+induction l;intros.
+- simpl. dd_ctx. exists x. split;auto. simpl in H. rewrite H. auto.
+- simpl. dd_ctx. exists x. split;auto. rewrite H. 
+  rewrite Failure_plus_fold. reflexivity. 
+Qed.
+
+Lemma In_mod_ACI_In_mod_LACI : forall l ll, In_mod_ACI (plus_fold l) (Failure::(map plus_fold (n_prod_list (f_extend ll)))) -> In_mod_LACI l (f_extend ll).
+Proof.
+induction l;intros. apply In_mod_LACI_f_extend. simpl in H.
+destruct (Contract_eq_dec a Failure).
+- subst. constructor. apply In_plus_Failure2 in H. apply IHl in H.
+  inversion H.
+  * subst.
+  exists l.
+  *
+constructor.
+-
+ simpl in H. unfold In_mod_ACI in H. d_ctx.
+
+Lemma In_mod_LACI_flatten : forall l ll, In_mod_LACI l ll -> In_mod_ACI (plus_fold l) (map plus_fold (n_prod_list (f_extend ll))).
+Proof.
+intros. induction H.
+- simpl. exists (Failure _+_ Failure). split; auto.
+- simpl. unfold In_mod_ACI. 
+induction ll;intros.
+- unfold is_FailureConf in*. destruct H. contradiction.
+- simpl. unfold is_FailureConf in*. simpl.
+
+
+
+
+
+Lemma AllDerivatives_plus_fold : forall (l : list Contract)(ll : list (list Contract)),
+is_FailureConf ll -> In_mod_LACI l ll -> In_mod_ACI (plus_fold l) (map plus_fold ll).
+Proof.
+induction l;intros.
+- simpl. unfold In_mod_LACI in *. exists Failure. simpl. split;auto.
+  unfold is_FailureConf in *. unfold In_mod_ACI.
+cofix IH.
+intros. constructor.
+- intros. rewrite plus_fold_derive. apply IH;auto.
+  intros.
+
+Definition In_mod_L (l : list Contract) (ll : list (list Contract)) := exists l', l' =L= l /\ In l' ll.
+
+Ltac dd_ctx := unfold In_mod_L,In_mod_R in *;destruct_ctx.
+
+Lemma In_mod_L_eq : forall l ll, In_mod_L l (l :: ll).
+Proof.
+intros. exists l;auto.
+Qed.
+
+Lemma In_mod_L_cons : forall l l' ll, In_mod_L l ll -> In_mod_L l (l' :: ll).
+Proof.
+intros. unfold In_mod_L in *. destruct H. destruct H. exists x.
+split;auto.
+Qed.
+
+Hint Resolve In_mod_L_eq In_mod_L_cons : dpDB.
+
+
+Lemma In_mod_L_app : forall ll0 ll1 l, In_mod_L l ll0 \/ In_mod_L l ll1 -> In_mod_L l (ll0++ll1).
+Proof.
+induction ll0;intros. simpl. destruct H.
+unfold In_mod_L in *.
+d_ctx. simpl in H0. contradiction. auto.
+inversion H.
+- dd_ctx. exists x. split;auto. apply in_or_app. now left.
+- dd_ctx. exists x. split;auto. apply in_or_app. now right.
+Qed.
+
+Fixpoint flatten (c : Contract) : list Contract :=
+match c with
+| c0 _+_ c1 => (flatten c0) ++ (flatten c1)
+| _ => [c]
+end.
+
+
+CoInductive AllFlatDerivatives : list Contract -> list (list Contract) -> Prop :=
+| AFD_fix l ll (H0: forall e, AllFlatDerivatives (flat_map (fun c => flatten (c/e)) l) ll) (H1 : In_mod_L l ll)  : AllFlatDerivatives l ll.
+
+Lemma All_AllFlat : forall c0 l, AllDerivatives c0 l -> AllFlatDerivatives (flatten c0) (map flatten l).
+Proof.
+cofix IH.
+intros. constructor.
+- intros. inversion H. subst.
+- 
+
 (*
 Lemma In_AllDerivatives_i_Trace_Derive : forall (c: Contract)(l : list Contract), 
 AllDerivatives c l -> (forall (s : Trace)(c_der : Contract), Trace_Derive c s c_der -> exists c', c' =R= c_der /\ In c' l).
 Proof.
 intros. generalize dependent c. induction s;intros.
-- inversion H0. subst. inversion H. destruct_ctx. exists x;auto.
+- inversion H0. subst. inversion H. d_ctx. exists x;auto.
 - inversion H0. inversion H. subst. eapply IHs. eapply H6. eauto.
+Qed.*)
+
+Lemma In_AllDerivatives : forall (c: Contract)(l : list Contract)(s : Trace), 
+AllDerivatives c l -> In_mod_R (c//s) l. 
+Proof.
+intros. generalize dependent c. induction s;intros.
+- inversion H. now simpl. 
+- inversion H. subst. eapply IHs. eauto.
 Qed.
 
+(*
 Lemma Trace_Derive_i_In_AllDerivatives : forall (c: Contract)(l : list Contract), 
 (forall (s : Trace)(c_der : Contract), Trace_Derive c s c_der -> exists c', c' =R= c_der /\ In c' l) -> AllDerivatives c l.
 Proof.
 cofix H_co.
 intros. constructor.
 - intros. apply H_co. intros. eapply H. constructor. eauto.
-- eauto with coDB.
-Qed.
+- eauto with icDB.
+Qed.*)
 
+(*
 Theorem AllDerivatives_iff : forall (c: Contract)(l : list Contract), 
 AllDerivatives c l <-> (forall (s : Trace)(c_der : Contract), Trace_Derive c s c_der -> exists c', c' =R= c_der /\ In c' l).
 Proof.
@@ -139,9 +333,17 @@ split;intros.
 - eapply Trace_Derive_i_In_AllDerivatives;eauto.
 Qed.*)
 
+(*
+Inductive OnlyDerivatives : Contract -> list Contract -> Prop :=
+| OD_nil c : OnlyDerivatives c [c]
+| OD_cons c c' l e (H: In_mod_R c' l) (H1: OnlyDerivatives c 
+*)
+
+
 Lemma AllDerivatives_Failure : AllDerivatives Failure [Failure].
 Proof.
 cofix IH. constructor;auto;simpl;auto.
+exists Failure;split;auto.
 Qed.
 
 Hint Resolve AllDerivatives_Failure : dpDB.
@@ -151,9 +353,8 @@ Hint Resolve AllDerivatives_Failure : dpDB.
 Lemma AllDerivatives_cons : forall (c c_der : Contract)(l : list Contract), AllDerivatives c l -> AllDerivatives c (c_der::l).
 Proof.
 cofix IH.
-intros. inversion H. 
-- constructor;auto. 
-- eapply AD_sub. eauto. apply IH. auto.
+intros. inversion H. constructor;auto.
+apply In_mod_R_cons;auto.
 Qed.
 
 Hint Resolve AllDerivatives_cons : dpDB.
@@ -162,7 +363,7 @@ Hint Resolve AllDerivatives_cons : dpDB.
 Lemma AllDerivatives_derive : forall c l e, AllDerivatives c l -> AllDerivatives (c/e) l.
 Proof.
 cofix IH. intros. inversion H.
-- destruct_ctx.
+- d_ctx.
 constructor; autodp. specialize H0 with e. destruct H0. auto.
 Qed.*)
 
@@ -186,7 +387,7 @@ cofix IH.
 intros.
 constructor; intros;simpl.
 - eq_event_destruct; autodp. 
-- now left.
+- exists (Event e). split;auto. 
 Qed.
 
 Hint Resolve AllDerivatives_Event : dpDB.
@@ -207,11 +408,6 @@ Global Transparent n_prod.
 
 Hint Unfold plus_prod : core.
 
-Fixpoint flatten (c : Contract) : list Contract :=
-match c with
-| c0 _+_ c1 => (flatten c0) ++ (flatten c1)
-| _ => [c]
-end.
 
 Lemma concat_n_prod : forall l ls, n_prod (l::ls) = plus_prod l ((n_prod ls)).
 Proof.
@@ -221,7 +417,7 @@ Qed.
 
 Lemma in_n_prod : forall c0 c1 l0 l1, In c0 l0 -> In c1 l1 -> In (c0 _+_ c1) (n_prod [l0; l1]).
 Proof. Admitted.
-
+(*
 Inductive List_AllDerivatives : list Contract -> list (list Contract) -> Prop :=
 | List_AllDerivatives_nil : List_AllDerivatives [] []
 | List_AllDerivatives_cons c l cs ls (H0 : AllDerivatives c l) (H1 : List_AllDerivatives cs ls) : List_AllDerivatives (c::cs) (l::ls).
@@ -229,7 +425,7 @@ Inductive List_AllDerivatives : list Contract -> list (list Contract) -> Prop :=
 Hint Constructors List_AllDerivatives : coDB.
 
 Lemma AllDerivatives_Flatten_iff : forall l ll, List_AllDerivatives l ll <-> AllDerivatives (plus_fold l) (n_prod ll).
-Proof. Admitted.
+Proof. Admitted.*)
 
 
 
@@ -239,13 +435,13 @@ induction c;intros.
 - exists Success. exists []. auto.
 - exists Failure. exists []. auto.
 - exists (Event e). exists []. auto.
-- destruct_ctx. exists x1. exists (x2 ++ (flatten c2)).
+- d_ctx. exists x1. exists (x2 ++ (flatten c2)).
   simpl. rewrite H0. now simpl.
 - exists (c1 _;_ c2). exists []. now simpl.
 - exists (Star c). exists []. now simpl.
 Qed.
 
-
+(*
 Lemma flatten_seq_derivative : forall c0 c1 e, flatten ((c0 _;_ c1)/ e) = [c0/e _;_ c1;o(c0)_;_(c1/e)].
 Proof.
 intros. now simpl.
@@ -257,7 +453,7 @@ induction s;intros. now simpl. simpl. rewrite derive_plus. simpl.
 rewrite derive_plus. simpl. rewrite derive_plus. simpl.
 rewrite app_nil_r. auto.
 Qed.
-
+*)
 
 
 Lemma Failure_trace_derive : forall s, Failure//s = Failure.
@@ -272,7 +468,7 @@ Proof.
 intros. o_destruct. rewrite H. now left. rewrite H. now right.
 Qed.
 
-
+(*
 Theorem flatten_seq_derive_shape : forall s c0 c1, exists l, (flatten ((c0 _;_ c1) // s)) = ((c0 // s) _;_ c1):: l /\
  Forall (fun c => exists c' s, c = (o c') _;_ (c1//s)) l.
 Proof.
@@ -280,10 +476,10 @@ induction s;intros.
 - simpl. exists []. split;auto.
 - rewrite flatten_seq_trace_derive. rewrite flatten_seq_derivative. simpl.
   rewrite app_nil_r. specialize IHs with (c0/a) c1 as IHs'.
-  specialize IHs with (o c0) (c1/a). destruct_ctx. rewrite H1. rewrite H.
+  specialize IHs with (o c0) (c1/a). d_ctx. rewrite H1. rewrite H.
   exists (x ++ o c0 // s _;_ c1 / a :: x0). split;auto.
   rewrite Forall_forall in *. intros. apply in_app_or in H3. destruct H3.
-  * apply H0 in H3. destruct_ctx. exists x2. now exists x3.
+  * apply H0 in H3. d_ctx. exists x2. now exists x3.
   * simpl in H3. destruct H3. 
     ** rewrite <- H3. destruct (o_or c0).
       *** rewrite H4. destruct s.
@@ -292,15 +488,538 @@ induction s;intros.
              now exists [a].
       *** rewrite H4. rewrite Failure_trace_derive. exists Failure.
           now exists [a].
-    ** apply H2 in H3. destruct_ctx. rewrite H3.
+    ** apply H2 in H3. d_ctx. rewrite H3.
        exists x2. now exists (a::x3).
-Qed.
+Qed.*)
+
+Definition seq_configurations (c1 : Contract) (l0 l1 : list Contract) := 
+ (repeat (Failure::l1) (length l1))++[map (fun c => c _;_ c1) l0].
 
 
 Inductive Flat_Seq_Derivative : Contract -> Contract -> list Contract -> Prop :=
 | FSD_Single c0 c1 s : Flat_Seq_Derivative c0 c1 [c0//s _;_ c1]
 | FSD_Cons_S c0 c1 l s (H: Flat_Seq_Derivative c0 c1 l) : Flat_Seq_Derivative c0 c1 ((Success _;_(c1//s))::l)
 | FSD_Cons_F c0 c1 l s (H: Flat_Seq_Derivative c0 c1 l) : Flat_Seq_Derivative c0 c1 ((Failure _;_(c1//s))::l).
+
+
+Lemma helper : forall s c0 e, (c0 // s) / e = c0 // (s ++ [e]).
+Proof.
+induction s;intros. now simpl.
+simpl. now rewrite IHs.
+Qed.
+
+Lemma helper2  : forall c e, c/e = c//[e].
+Proof. auto. Qed.
+
+
+Lemma Flat_Seq_Derivative_closed : forall c0 c1 l e, Flat_Seq_Derivative c0 c1 l -> 
+Flat_Seq_Derivative c0 c1 (flat_map (fun c => flatten (c/e)) l).
+Proof.
+intros. induction H.
+- simpl. rewrite helper2. o_destruct; rewrite H.
+  all: constructor; rewrite helper; constructor.
+- simpl. rewrite o_Success. rewrite helper. constructor. constructor.
+  auto.
+- simpl. rewrite o_Failure. rewrite helper. constructor. constructor.
+  auto.
+Qed.
+
+Lemma plus_fold_flatten : forall c , plus_fold (flatten c) =R= c.
+Proof.
+induction c;intros;simpl;auto_rwd.
+rewrite c_eq_iff. setoid_rewrite plus_fold_app.
+rewrite <- c_eq_iff. rewrite IHc1.
+now rewrite IHc2.
+Qed.
+
+
+Lemma plus_fold_derive_flatten : forall (l : list Contract) (e : EventType), (plus_fold l) / e =R= plus_fold (flat_map (fun c => (flatten (c/e))) l).
+Proof.
+induction l;intros.
+- now simpl.
+- simpl. rewrite c_eq_iff. setoid_rewrite plus_fold_app.
+  rewrite <- c_eq_iff. rewrite IHl. now rewrite plus_fold_flatten.
+Qed.
+
+Lemma Flat_Seq_Derivative_repeat_Failure : forall n c0 c1 l , Flat_Seq_Derivative c0 c1 l -> Flat_Seq_Derivative c0 c1  ((repeat (Failure _;_ (c1)) n)++l).
+Proof.
+induction n;intros.
+- now simpl.
+- simpl. assert (HA: c1 = c1 // []). { auto. } rewrite HA. constructor. auto.
+Qed.
+
+Lemma Flat_Seq_Derivative_repeat_Success : forall n c0 c1 l , Flat_Seq_Derivative c0 c1 l -> Flat_Seq_Derivative c0 c1  ((repeat (Success _;_ (c1)) n)++l).
+Proof.
+induction n;intros.
+- now simpl.
+- simpl. assert (HA: c1 = c1 // []). { auto. } rewrite HA. constructor. auto.
+Qed.
+
+Lemma plus_fold_repeat_failure : forall n c1, plus_fold (repeat (Failure _;_ c1) n) =R= Failure.
+Proof.
+induction n;intros;simpl;auto.
+rewrite IHn. auto_rwd.
+Qed.
+
+Equations n_prod_list (A:Type)(ll : list (list A)) : list (list A) by wf (length ll) lt :=
+n_prod_list [] := [[]];
+n_prod_list (l::ll') := map (fun p => (fst p)::(snd p)) (list_prod l (n_prod_list (ll'))).
+Global Transparent n_prod_list.
+
+Eval compute in (n_prod_list [[0;1];[2;3]]).
+
+Eval compute in (n_prod_list []).
+
+Check incl.
+
+Check In_mod_R.
+
+(*
+Lemma n_prod_list_app : forall (A:Type)(ll0 ll1 : list (list A)), 
+n_prod_list (ll0++ll1) = n_prod_list((n_prod_list ll0)++(n_prod_list ll1)).
+Proof.
+induction ll0;intros.
+- simpl. simp n_prod_list. simpl.*)
+
+(*
+Inductive In_N_Prod_List : list Contract -> list (list Contract) -> Prop :=
+| INPL_nil : In_N_Prod_List [] []
+| INPL_cons l ll e l' (H0: In_N_Prod_List l ll) (H1: In e l') : In_N_Prod_List (e::l) (l'::ll).
+*)
+
+ 
+(*Nicer to use an inductive definition because of the 
+  generated induction principle, and avoiding to deal with out of bounds
+  cases*)
+(*
+
+Lemma n_prod_list_singleton : forall (A : Type)(l : list A), n_prod_list [l] = map (fun e => [e]) l.
+Proof.
+intros. destruct l. funelim (n_prod_list [l]). induction l;intros.
+- contradiction. 
+- simp n_prod_list. simpl. simpl. f_equal.*)
+
+
+Lemma in_n_prod_list_extend : forall (l l' : list Contract) e(ll : list (list Contract)),
+ In l (n_prod_list ll) -> In e l' -> In (e::l) (n_prod_list (l'::ll)).
+Proof.
+induction l;intros.
+- simp n_prod_list. rewrite in_map_iff.
+  exists (e,[]). split;auto. apply in_prod;auto.
+- simp n_prod_list. rewrite in_map_iff.
+  exists (e,a::l). split;auto. apply in_prod;auto.
+Qed.
+
+Lemma in_n_prod_cons : forall (l l' : list Contract) e(ll : list (list Contract)),
+ In (e::l) (n_prod_list (l'::ll)) -> In e l' /\ In l (n_prod_list ll).
+Proof.
+intros. simp n_prod_list in H. rewrite in_map_iff in H.
+d_ctx. inversion H. subst. destruct x.
+rewrite in_prod_iff in H0. simpl.
+destruct H0;auto.
+Qed.
+
+Lemma in_n_prod_iff : forall (l l' : list Contract) e(ll : list (list Contract)),
+ In (e::l) (n_prod_list (l'::ll)) <-> In e l' /\ In l (n_prod_list ll) .
+Proof.
+split;intros. auto using in_n_prod_cons.
+destruct H. auto using in_n_prod_list_extend.
+Qed.
+
+Lemma in_n_prod_app : forall (l l' : list Contract) (ll ll' : list (list Contract)),
+ In l (n_prod_list ll) -> In l' (n_prod_list ll')  -> In (l++l') (n_prod_list (ll++ll')).
+Proof.
+induction l;intros;simpl.
+- destruct ll. simpl in H. destruct H;try contradiction.
+  auto. simp n_prod_list in H. rewrite in_map_iff in H.
+  d_ctx. discriminate.
+- destruct ll. simpl. simpl in H. destruct H;try contradiction. 
+  discriminate. rewrite <- app_comm_cons. rewrite in_n_prod_iff. 
+  rewrite in_n_prod_iff in H. destruct H;auto.
+Qed.
+
+Lemma in_n_prod_repeat : forall (A:Type) (n:nat) (e:A) (l:list A) ,
+ In e l-> In (repeat e n) (n_prod_list (repeat l n)).
+Proof.
+intro. induction n;intros;simpl. now left.
+apply IHn in H as H'. simp n_prod_list.
+ rewrite in_map_iff. exists (e,repeat e n).
+split;auto. rewrite in_prod_iff. split;auto.
+Qed.
+
+Print or.
+
+
+(*
+Lemma in_n_prod_list2 : forall (l : list Contract)(ll : list (list Contract)),
+In l (n_prod_list ll) -> In_N_Prod_List l ll.
+Proof.
+induction l;intros.
+- destruct ll.  constructor.
+  simp n_prod_list in H. rewrite in_map_iff in H.
+  d_ctx. discriminate.
+- destruct ll. simp n_prod_list in H. simpl in H.
+  destruct H. discriminate. contradiction.
+  eapply in_n_prod_list3 in H; destruct H.
+  constructor;eauto.
+Qed.*)
+(*
+Lemma in_n_prod_list : forall (l : list Contract)(ll : list (list Contract)),
+In_N_Prod_List l ll -> In l (n_prod_list ll).
+Proof.
+intros. induction H.
+- simpl. now left.
+-
+ constructor.*)
+
+(*
+(default:A),
+(forall l', In l' ll -> ~(In default l')) ->
+(forall n, In (nth n l default) (nth n ll [default])) ->
+In l (n_prod_list ll).
+Proof.
+intros. funelim (n_prod_list ll).
+- simpl. specialize H0 with 0. simpl in H0.
+  destruct H0;try contradiction. destruct l;auto.
+  simpl in H0. induction l.
+- intros. funelim (n_prod_list ll).
+  *  simpl. now left.
+  * specialize H1 with 0. simpl in H1. apply H0 in H1;auto. contradiction.
+- intros. 
+ simpl. now left.
+  *
+- simpl. left. destruct l;auto.
+  simpl in H. destruct n. unfold n_prod_list. 
+*)
+(*
+Lemma InAllDerivatives : forall c l, AllDerivatives c l -> In_mod_R c l.
+Proof.
+intros. inversion H.
+- exists c. split;auto.
+-
+
+Lemma InAllDerivatives : forall s c l, AllDerivatives c l -> In_mod_R (c//s) l.
+Proof.
+induction s;intros.
+- simpl. inversion H. 
+intros inversion H.
+-
+*)
+Lemma AllDerivatives_nil : forall c, AllDerivatives c [] -> False.
+Proof.
+intros. inversion H. unfold In_mod_R in H1. d_ctx.
+simpl in H4. contradiction.
+Qed.
+
+
+
+Lemma plus_list_equivalence_incl : forall (l0 l1 : list Contract), (forall c, In_mod_R c l0 <-> In_mod_R c l1) <-> l0 =L= l1.
+Proof. Admitted.
+
+Lemma plus_list_eq_repeat_failure : forall n l0 l1, l0 =L= l1 -> l0 =L= repeat Failure n ++ l1.
+Proof.
+induction n;intros.
+- now simpl.
+- simpl. rewrite IHn;eauto. auto_rwd.
+Qed.
+
+Lemma repeat_failure_nil : forall n , repeat Failure n =L= [].
+Proof.
+induction n;intros;simpl;auto_rwd.
+auto.
+Qed.
+
+
+(*
+Lemma In_mod_L_n_prod_iff : forall (l l' : list Contract) e(ll : list (list Contract)),
+ In (e::l) (n_prod_list (l'::ll)) <-> In e l' /\ In l (n_prod_list ll) .
+Proof.
+split;intros. auto using in_n_prod_cons.
+destruct H. auto using in_n_prod_list_extend.
+Qed.*)
+
+
+Lemma In_mod_L_n_prod_list_extend : forall (ll : list (list Contract)) c(l  : list (Contract)),
+ In_mod_L l (n_prod_list ll) -> In c l -> In_mod_L (c::l) (n_prod_list (l::ll)).
+Proof. Admitted.
+(*intros. Check in_n_prod_list_extend.
+dd_ctx. eapply in_n_prod_list_extend in H1.
+exists (c::l). split;auto. eauto. eauto.
+Qed.*)
+(*Continue from here in_n_prod_cons*)
+(*
+Lemma In_mod_L_n_prod_cons : forall (ll : list (list Contract)) c(l l' : list (Contract)),
+ In_mod_L (c::l) (n_prod_list (l'::ll)) -> In c l' /\ In_mod_L l (n_prod_list ll).
+Proof.
+intros. simp n_prod_list in H. dd_ctx. rewrite in_map_iff in H0.
+dd_ctx. inversion H0. subst. split.
+- destruct x0. rewrite in_prod_iff in H1. simpl.
+destruct H1;auto. exists c. split;auto.
+- destruct x0. rewrite in_prod_iff in H1. simpl.
+  exists l. destruct H1. split;auto.
+Qed.*)
+(*
+Lemma In_mod_L_n_prod_iff : forall (ll : list (list Contract)) c(l l' : list (Contract)),
+ In_mod_L (c::l) (n_prod_list (l'::ll)) <-> In_mod_R c l' /\ In_mod_L l (n_prod_list ll).
+Proof.
+split;intros. auto using In_mod_L_n_prod_cons.
+destruct H. eapply In_mod_L_n_prod_list_extend. eauto using In_mod_L_n_prod_list_extend.
+Qed.
+
+
+
+Lemma in_n_prod_repeat : forall (A:Type) (n:nat) (e:A) (l:list A) ,
+ In e l-> In (repeat e n) (n_prod_list (repeat l n)).
+Proof.
+intro. induction n;intros;simpl. now left.
+apply IHn in H as H'. simp n_prod_list.
+ rewrite in_map_iff. exists (e,repeat e n).
+split;auto. rewrite in_prod_iff. split;auto.
+Qed.*)
+
+Lemma In_mod_L_n_prod_app : forall (l l' : list Contract) (ll ll' : list (list Contract)),
+ In_mod_L l (n_prod_list ll) -> In_mod_L l' (n_prod_list ll')  -> In_mod_L (l++l') (n_prod_list (ll++ll')).
+Proof. Admitted.
+(*
+induction l;intros;simpl.
+- destruct ll. simp n_prod_list in H.
+  destruct H;try contradiction.
+  auto. simp n_prod_list in H. rewrite in_map_iff in H.
+  d_ctx. discriminate.
+- destruct ll. dd_ctx. simpl in H2. destruct H2;try contradiction.
+  discriminate. rewrite <- app_comm_cons. rewrite in_n_prod_iff. 
+  rewrite in_n_prod_iff in H. destruct H;auto.
+Qed.*)
+
+Lemma Flat_Seq_Derivative_sc : forall c0 c1 l l0 l1, AllDerivatives c0 l0 -> AllDerivatives c1 l1 ->
+In l (n_prod_list (seq_configurations c1 l0 l1)) -> Flat_Seq_Derivative c0 c1 l.
+Proof. Admitted.
+
+Lemma in_l_list_eq : forall (c : Contract)(l : list Contract), In c l -> c::l =L= l.
+Proof.
+Admitted.
+
+Lemma test_occ : forall c c1 l l0 l1,
+In_mod_L l (n_prod_list (seq_configurations c1 l0 l1)) -> In c l1 -> (~ In c l) -> exists c', In c' (Failure::l1) /\  count_occ Contract_eq_dec l c' > 1.
+Proof.
+Admitted.
+
+Lemma reduce_occ : forall (l : list Contract) c, repeat c ((count_occ Contract_eq_dec l c)) ++ (remove Contract_eq_dec c l) =L= l.
+Proof.
+induction l;intros;simpl.
+- auto.
+- destruct (Contract_eq_dec a c).
+  * destruct (Contract_eq_dec c a).
+    ** simpl. subst. simpl in IHl. auto_rwd. specialize IHl with c.
+       apply c_eq_plus_morphism;auto.
+    ** simpl. subst. contradiction.
+  * destruct (Contract_eq_dec c a).
+    ** simpl. subst. contradiction.
+    ** rewrite c_eq_iff. setoid_rewrite plus_fold_app. simpl.
+       setoid_rewrite <- plus_assoc. 
+       rewrite <- c_eq_iff. rewrite <- IHl.
+       rewrite (plus_comm_ceq _ a).
+       rewrite c_eq_iff.  repeat  setoid_rewrite  plus_assoc. 
+       rewrite <- c_eq_iff. 
+ auto_rwd. apply c_eq_plus_morphism;auto.
+       rewrite c_eq_iff. setoid_rewrite plus_fold_app.
+       rewrite <- c_eq_iff. auto_rwd. apply c_eq_plus_morphism; eauto.
+Qed.
+
+Lemma list_eq_cons_comm : forall l c0 c1, c0 :: c1 :: l =L= c1:: c0 ::l.
+Proof.
+induction l;intros.
+- simpl. auto_rwd.
+- simpl. specialize IHl with c1 a. simpl in IHl. rewrite IHl.
+  repeat rewrite (plus_comm_ceq a _ ). repeat rewrite <- plus_assoc_ceq.
+  apply c_eq_plus_morphism;auto. now rewrite (plus_comm_ceq c1).
+Qed.
+
+
+Lemma reduce_occ2 : forall (l : list Contract) c, c::(remove Contract_eq_dec c l) =L= c::l.
+Proof.
+induction l;intros. auto.
+simpl.
+destruct (Contract_eq_dec c a).
+- subst. specialize IHl with a. simpl in IHl. rewrite IHl.
+  rewrite <- plus_assoc_ceq. auto_rwd.
+- simpl. rewrite <- (plus_assoc_ceq c). rewrite (plus_comm_ceq _ a).
+  rewrite plus_assoc_ceq. specialize IHl with c as IHl'. simpl in IHl'.
+   rewrite IHl'. auto_rwd. rewrite plus_comm_ceq.
+   rewrite plus_assoc_ceq. 
+ apply c_eq_plus_morphism;auto. apply plus_comm_ceq.
+Qed.
+(*
+
+
+Lemma flat_seq_in_seq_configuration : forall c c1 l l0 l1,
+In c l1 -> In_mod_L l (n_prod_list (seq_configurations c1 l0 l1)) -> In_mod_L (c::l) (n_prod_list (seq_configurations c1 l0 l1)).
+Proof.
+intros. dd_ctx. destruct (in_dec Contract_eq_dec c l).
+- dd_ctx. exists x. rewrite in_l_list_eq;auto.
+- eapply test_occ in H0;eauto. dd_ctx. apply reduce_occ in H1.
+ split;auto.
+
+*)
+
+Lemma flat_seq_in_seq_configuration : forall c0 c1 l l0 l1, AllDerivatives c0 l0 -> AllDerivatives c1 l1 -> Flat_Seq_Derivative c0 c1 l -> 
+In_mod_L l (n_prod_list (seq_configurations c1 l0 l1)).
+Proof. 
+intros. induction H1. 
+- unfold seq_configurations.
+  apply In_AllDerivatives with (s:=s) in H as H9.
+  rewrite <- (app_nil_l [c0 // s _;_ c1]).
+  apply In_mod_L_n_prod_app.
+  unfold In_mod_L. exists (repeat Failure (length l1)). split.
+  apply repeat_failure_nil. apply in_n_prod_repeat. auto.
+  simp n_prod_list. unfold In_mod_L. destruct H9.
+  exists [x _;_ c1]. split;auto. simpl. auto_rwd. destruct H1.
+  now rewrite H1. rewrite in_map_iff. exists (x _;_ c1,[]).
+   simpl. split;auto. rewrite in_prod_iff. split;auto.
+   rewrite in_map_iff. exists x. destruct H1. split;auto.
+Admitted.
+(*
+ rewrite H1. simpl.
+  symmetry.
+  symmetry. split;auto. simpl. auto_rwd. 
+  apply In_mod_L_app.
+  exists ((repeat Failure (length l1))++[c0//s _;_ c1]).
+  split. symmetry. now apply plus_list_eq_repeat_failure.
+  
+  * apply in_n_prod_app.
+    ** apply in_n_prod_repeat;auto.
+    ** simp n_prod_list. rewrite in_map_iff.
+       exists (c0//s _;_ c1,[]). split;auto. rewrite in_prod_iff. simpl.
+       split;auto. rewrite in_map_iff. exists x. split;auto.
+  * apply plus_list_eq_repeat_failure. simpl.
+    rewrite H1. auto_rwd.
+- pose proof H as H'. pose proof H0 as H0'. apply IHFlat_Seq_Derivative in H.
+  apply IHFlat_Seq_Derivative in H0. all:auto.
+  apply In_AllDerivatives with (s:=s) in H0' as H9.
+  d_ctx. exists x1. split;auto. intros. simpl in H6.
+  destruct H6;auto. subst. exists x.  split;auto.
+  rewrite H2. auto_rwd. auto.
+    d_ctx. exists x. apply In_mod_R_app.
+      *** simpl.
+       exists (c0 // s _;_ c1,[]). split;auto.
+       simpl.
+       rewrite in_prod_iff. split;auto. rewrite in_map_iff.
+       exists (c0//s). split;auto.*)
+
+Lemma seq_configuration_in_flat_seq : forall c0 c1 l l0 l1, Flat_Seq_Derivative c0 c1 l -> exists l', In l' (n_prod_list (seq_configurations c1 l0 l1)) /\
+(forall c, In c l -> In_mod_R c l').
+Proof. Admitted.
+
+
+Lemma in_seq_configuration_iff : forall c0 c1 l l0 l1, Flat_Seq_Derivative c0 c1 l -> exists l', In l' (n_prod_list (seq_configurations c1 l0 l1)) /\
+(forall c, In c l -> In_mod_R c l') /\ (forall c, In c l' -> In_mod_R c l).
+Proof. Admitted.
+
+
+
+Lemma Flat_seq_in_conf : forall c0 c1 l l0 l1, Flat_Seq_Derivative c0 c1 l -> exists l', In l' (n_prod_list (seq_configurations c1 l0 l1)) 
+/\ plus_fold l =R= plus_fold l' /\ Flat_Seq_Derivative c0 c1 l'.
+Proof. Admitted.
+
+Lemma in_n_prod_list_plus_fold : forall l l_conf, In l (n_prod_list l_conf) 
+-> In (plus_fold l) (map plus_fold (n_prod_list l_conf)).
+Proof. Admitted.
+
+Lemma All_Derivatives_Flat_Seq_test : forall c0 c1 l l0 l1, 
+AllDerivatives (plus_fold l) (map plus_fold (n_prod_list (seq_configurations c1 l0 l1))).
+Proof.
+
+
+Lemma All_Derivatives_Flat_Seq : forall c0 c1 l l0 l1, Flat_Seq_Derivative c0 c1 l -> AllDerivatives c0 l0
+-> AllDerivatives c1 l1 -> AllDerivatives (plus_fold l) (map plus_fold (n_prod_list (seq_configurations c1 l0 l1))).
+Proof.
+cofix IH.
+intros. apply Flat_seq_in_conf with (l0:=l0) (l1:=l1) in H as H'.
+d_ctx. eapply AD_sub. symmetry. eauto. econstructor.
+- intros. eapply AD_sub. symmetry. eapply plus_fold_derive_flatten.
+  eapply IH;eauto. apply Flat_Seq_Derivative_closed;auto. 
+- apply in_n_prod_list_plus_fold;auto.
+Qed.
+
+Lemma All_Derivatives_Seq : forall c0 c1 l0 l1, AllDerivatives c0 l0 -> AllDerivatives c1 l1
+-> AllDerivatives ( c0 _;_c1) (map plus_fold (n_prod_list (seq_configurations c1 l0 l1))).
+Proof.
+intros. eapply AD_sub with (c0 _;_ c1 _+_ Failure);auto_rwd.
+assert (HA: c0 _;_ c1 _+_ Failure = plus_fold [c0 _;_ c1]). { now simpl. }
+rewrite HA. eapply All_Derivatives_Flat_Seq;eauto.
+assert (HA2: c0 _;_ c1 = c0//[] _;_ c1). { auto. } rewrite HA2.
+constructor.
+Qed.
+ 
+
+Lemma Flat_Seq_Derivative_length : forall c0 c1 l1 l, AllDerivatives c1 l1 -> Flat_Seq_Derivative c0 c1 l -> exists l', Flat_Seq_Derivative c0 c1 l' /\
+ plus_fold l =R= plus_fold l' /\ length l' = length l1 + 1.
+Proof.
+intros. induction H0.
+- exists ((repeat (Failure _;_ c1) (length l1))++[(c0//s _;_ c1)]). split.
+  * apply Flat_Seq_Derivative_repeat_Failure. constructor.
+  * split.
+    ** rewrite c_eq_iff. setoid_rewrite plus_fold_app.
+       rewrite <- c_eq_iff. simpl. rewrite plus_fold_repeat_failure.
+       auto_rwd.
+    ** simpl. rewrite app_length. rewrite repeat_length. auto.  
+- apply IHFlat_Seq_Derivative in H. d_ctx. (*Idempotence argument*)
+ Admitted.
+
+
+
+
+
+
+
+
+
+Lemma AllDerivatives_Seq : forall (c0 c1 c : Contract)(l0 l1 : list Contract) l l', l=c::l' -> AllDerivatives c0 l0 -> AllDerivatives c1 l1 -> 
+AllDerivatives (c0 _;_ c1) (n_prod (seq_configurations c1 l0 l1)).
+Proof. 
+cofix IH.
+intros. constructor.
+- intros. simpl. constructor. intros. simpl. cofix IH_plus. unfold seq_closure. rewrite concat_n_prod. 
+apply AllDerivatives_Plus.
+  * cofix IH_plus. constructor.
+    ** intros. simpl.
+
+ 
+
+
+
+
+
+
+
+
+
+
+
+
+
+
+
+
+
+
+
+
+
+
+
+
+
+
+
+
+
+
+
+
+
+
+
 
 (*
 Inductive Flat_Seq_Derivative : Contract -> Contract -> list Contract -> Prop :=
@@ -322,16 +1041,7 @@ intros. constructor.
 
 Lemma in_AllDerivatives: forall c0 l0 c e, AllDerivatives c0 l0 -> In_mod_R c l0 -> In_mod_R (c/e) l0.
 Proof.
-intros. unfold In_mod_R in H0. destruct_ctx. inversion H. unfold In_mod_R in *)
-
-Lemma helper : forall s c0 e, (c0 // s) / e = c0 // (s ++ [e]).
-Proof.
-induction s;intros. now simpl.
-simpl. now rewrite IHs.
-Qed.
-
-Lemma helper2  : forall c e, c/e = c//[e].
-Proof. auto. Qed.
+intros. unfold In_mod_R in H0. d_ctx. inversion H. unfold In_mod_R in *)
 
 Lemma flatten_cons : forall c, exists c' l, c'::l = flatten c .
 Proof. Admitted.
@@ -361,7 +1071,7 @@ induction l;intros. split.
 - destruct s. simpl in *. inversion H. auto. simpl in H.
   rewrite derive_plus in H. simpl in H.
   destruct (flatten_cons ((c0 / e _;_ c1) // s)).
-  destruct (flatten_cons (((o c0 _;_ c1 / e) // s))). destruct_ctx.
+  destruct (flatten_cons (((o c0 _;_ c1 / e) // s))). d_ctx.
   rewrite H0 in H. rewrite H1 in H. simpl in H. inversion H.
   Search ([] = _). apply app_cons_not_nil in H4. contradiction.
 - auto.
@@ -377,7 +1087,7 @@ induction s;intros.
 - simpl. exists (c0 _;_ c1). exists []. split;auto.
 - simpl. rewrite derive_plus. simpl.
   specialize IHs with (c0/a) c1.
-  destruct_ctx. exists x. exists (x0 ++ (flatten ((o c0 _;_ c1 / a) // s))).
+  d_ctx. exists x. exists (x0 ++ (flatten ((o c0 _;_ c1 / a) // s))).
   split;auto.
   * now rewrite <- H.
   * split;auto. simpl. pose proof H1. rewrite Forall_forall in H1. rewrite Forall_forall.
@@ -390,37 +1100,13 @@ Lemma Flat_Seq_Derivative_closed : forall c0 c1 l, Forall (fun c => Failure _;_ 
 Flat_Seq_Derivative c0 c1 (flat_map (fun c => flatten (c/e)) l).
 Proof.
 
-Lemma Flat_Seq_Derivative_closed : forall c0 c1 l e, Flat_Seq_Derivative c0 c1 l -> 
-Flat_Seq_Derivative c0 c1 (flat_map (fun c => flatten (c/e)) l).
-Proof.
-intros. induction H.
-- simpl. rewrite helper2. o_destruct; rewrite H.
-  all: constructor; rewrite helper; constructor.
-- simpl. rewrite o_Success. rewrite helper. constructor. constructor.
-  auto.
-- simpl. rewrite o_Failure. rewrite helper. constructor. constructor.
-  auto.
-Qed.
-
-Definition seq_configurations (c1 : Contract) (l0 l1 : list Contract) := 
- (repeat (Failure::l1) (length l1))++[map (fun c => c _;_ c1) l0].
-
-Lemma plus_fold_flatten : forall c , plus_fold (flatten c) =R= c.
-Proof.
-induction c;intros;simpl;auto_rwd.
-rewrite c_eq_iff. setoid_rewrite plus_fold_app.
-rewrite <- c_eq_iff. rewrite IHc1.
-now rewrite IHc2.
-Qed.
 
 
-Lemma plus_fold_derive_flatten : forall (l : list Contract) (e : EventType), (plus_fold l) / e =R= plus_fold (flat_map (fun c => (flatten (c/e))) l).
-Proof.
-induction l;intros.
-- now simpl.
-- simpl. rewrite c_eq_iff. setoid_rewrite plus_fold_app.
-  rewrite <- c_eq_iff. rewrite IHl. now rewrite plus_fold_flatten.
-Qed.
+
+
+
+
+
 
 Lemma in_seq_configurations : forall c0 c1 l l0 l1, Flat_Seq_Derivative c0 c1 l -> AllDerivatives c0 l0
 -> AllDerivatives c1 l1 -> In_mod_R (plus_fold l) (n_prod (seq_configurations c1 l0 l1)).
@@ -447,7 +1133,7 @@ intros. econstructor.
   * eapply Flat_Seq_Derivative_closed. unfold seq_configurations.
 
 
-Ltac in_forall HF HIn := rewrite Forall_forall in HF; apply HF in HIn;destruct_ctx;subst.
+Ltac in_forall HF HIn := rewrite Forall_forall in HF; apply HF in HIn;d_ctx;subst.
 
 Lemma flatten_seq_derive_FSD : forall c0 c1 c_der s l, Flat_Seq_Derivative c0 c1 s (length s) l -> 
  In c_der (flatten ((c0 _;_ c1) // s)) <-> ((exists c', c' =R= c_der /\ In c' l) \/ c_der =R= Failure).
@@ -469,7 +1155,7 @@ Proof.
 cofix IH.
 intros. constructor. intros; simpl.
 - inversion H. eapply IH. inversion H. eauto. inversion H0. eauto.
-- inversion H0. destruct_ctx. subst. exists x. split;auto. now rewrite H2.
+- inversion H0. d_ctx. subst. exists x. split;auto. now rewrite H2.
 Qed.
 
 Lemma AllDerivatives_sub_iff : forall c0 c1 l, c0 =R= c1 -> AllDerivatives c0 l <-> AllDerivatives c1 l.
@@ -495,7 +1181,7 @@ Hint Resolve AllDerivatives_Plus : coDB.*)
 Lemma AllDerivatives_plus_plus_fold : forall (c0 c1 : Contract)(l : list Contract), AllDerivatives (c0 _+_ c1) l -> 
  AllDerivatives (plus_fold [c0;c1] ) l.
 Proof. c_eq_tac. auto_rwd. inversion H. apply AllDerivatives_sub with(c0:= c0/e _+_ c1/e);
-       simpl in H0. auto_rwd. auto. inversion H. destruct_ctx.
+       simpl in H0. auto_rwd. auto. inversion H. d_ctx.
        exists x. auto_rwd.
 Qed.
 
@@ -503,7 +1189,7 @@ Lemma AllDerivatives_plus_fold_plus : forall (c0 c1 : Contract)(l : list Contrac
  AllDerivatives (plus_fold [c0;c1] ) l -> AllDerivatives (c0 _+_ c1) l .
 Proof.
 c_eq_tac. inversion H. simpl in H0.  apply AllDerivatives_sub with(c0:= c0/e _+_ (c1/e _+_ Failure));
-simpl. auto_rwd. auto. inversion H. destruct_ctx. exists x. simpl in H1.
+simpl. auto_rwd. auto. inversion H. d_ctx. exists x. simpl in H1.
 split;auto. now autorewrite with coDB in H1.
 Qed.
 
@@ -515,7 +1201,7 @@ Qed.
 
 
 Lemma AllDerivatives_comm : forall c0 c1 l, AllDerivatives (c0 _+_ c1) l -> AllDerivatives (c1 _+_ c0) l.
-Proof. c_eq_tac. inversion H;eauto. inversion H. destruct_ctx.
+Proof. c_eq_tac. inversion H;eauto. inversion H. d_ctx.
        exists x. split;auto. rewrite H1. auto with coDB.
 Qed.
 
@@ -535,10 +1221,7 @@ Qed.
 
 Definition failure_seq_list l := map (fun l => Failure::l) (repeat l (length l)).
 
-Lemma AllDerivatives_nil : forall c, AllDerivatives c [] -> False.
-Proof.
-intros. inversion H. destruct_ctx. simpl in H4. contradiction.
-Qed.
+
 
 Search ((o _)/_).
 Locate o_derive.
@@ -561,7 +1244,7 @@ intros. constructor;intros.
   autorewrite with icDB. closure_sub (o c0 _;_ c1 / e);auto_rwd.
   apply IH. Guarded. Guarded.   inversion H. eauto.  
 - destruct (o_or c0); destruct H0;rewrite H0.
-  * inversion H. destruct_ctx. exists x.
+  * inversion H. d_ctx. exists x.
     split;auto_rwd. auto.
   * exists Failure. split;auto_rwd. auto.
 Qed.*)
@@ -629,12 +1312,12 @@ Qed.
 Theorem In_mod_ACI_cons : forall (c c' : Contract) (l : list Contract), In_mod_ACI c (c'::l) <-> c' =ACI= c \/ In_mod_ACI c l.
 Proof.
 split;intros.
-- rewrite In_mod_ACI_iff_In in H. destruct_ctx. induction H.
+- rewrite In_mod_ACI_iff_In in H. d_ctx. induction H.
   * subst. now left.
   * right. rewrite In_mod_ACI_iff_In. exists x. split;auto.
 - destruct H.
   * rewrite In_mod_ACI_iff_In. exists c'. split;auto using in_eq.
-  * rewrite In_mod_ACI_iff_In in *. destruct_ctx. exists x.
+  * rewrite In_mod_ACI_iff_In in *. d_ctx. exists x.
     split;auto using in_cons,in_eq.
 Qed. *)
 
@@ -674,7 +1357,7 @@ Theorem Failure_derive_i_in_flatten_seq : forall s c1, exists c_der, c_der =b= F
 Proof.
 induction s;intros.
 - exists (Failure _;_ c1). simpl. split;autoM.
-- simpl. auto_rwd. simpl. specialize IHs with c1 as IHs'. destruct_ctx. exists x.
+- simpl. auto_rwd. simpl. specialize IHs with c1 as IHs'. d_ctx. exists x.
   split;autoM. rewrite in_app_iff.  now left. 
 Qed.
 
@@ -686,7 +1369,7 @@ Definition bool_equiv_lists (l0 l1 : list Contract) := bool_incl_lists l0 l1 /\ 
 Lemma test : forall s c, bool_equiv_lists (flatten ((Failure _;_ c) // s)) [Failure].
 Proof.
 intros. unfold bool_equiv_lists,bool_incl_lists. split.
-- intros. pose proof Failure_derive_i_in_flatten_seq s c. destruct_ctx.
+- intros. pose proof Failure_derive_i_in_flatten_seq s c. d_ctx.
   exists x.
 Admitted.
 
@@ -715,7 +1398,7 @@ induction s;intros.
   * apply IHs in H. destruct H.
     ** now left.
     ** destruct H. 
-      *** destruct_ctx. subst. right. left. exists (a::x). exists x0.
+      *** d_ctx. subst. right. left. exists (a::x). exists x0.
           split;auto.
       *** right. right. auto.
   * apply in_flatten_seq_o_derive in H. destruct H;auto. 
@@ -738,12 +1421,12 @@ Proof.
 intro. 
 induction s;intros;simpl.
 - split;intros. destruct H;try contradiction. inversion H. subst. now left.
-  destruct H. inversion H. now left. destruct_ctx. contradiction.
+  destruct H. inversion H. now left. d_ctx. contradiction.
 - split;intros.
   * rewrite derive_plus in H. simpl in H. apply in_app_or in H. destruct H.
     ** apply IHs in H. destruct H.
       *** now left.
-      *** destruct_ctx. destruct H0.
+      *** d_ctx. destruct H0.
         **** subst. right. split.  intro H2.  discriminate. split. now left. 
              exists (S x). exists x0. now simpl.
         **** subst. right. split. intro H2. discriminate. split. now right.
@@ -754,7 +1437,7 @@ induction s;intros;simpl.
           destruct s. simpl. now left. simpl. rewrite Failure_trace_derive.
           now right. rewrite H0. rewrite Failure_trace_derive. now right.
           exists 0. exists 1. simpl. auto.
-      *** destruct_ctx. subst. destruct H0.
+      *** d_ctx. subst. destruct H0.
         **** rewrite H0. right. split;auto. intro H2. discriminate.
              split. now left. exists 0. exists x0.
  Check trace_derive_failure. rewrite  r simpl; left.
@@ -763,7 +1446,7 @@ induction s;intros;simpl.
   exists 1. now simpl. split. destruct H. inversion H. subst.
   destruct (o_or c0). rewrite H0. right. now left. rewrite H0. right. right. auto.
   inversion H. inversion H. inversion H0. subst. exists 0. now simpl.
-  inversion H0. destruct_ctx. destruct H. destruct x.
+  inversion H0. d_ctx. destruct H. destruct x.
   * simpl in H0. subst. intuition. auto.
  subst. destruct H;subst. simpl. now right. susbt. 
  rewrite H.
@@ -778,12 +1461,12 @@ c_der0 = Failure /\ exists n_low n_high, c_der1 = c1//(skipn n_low (firstn n_hig
 Proof.
 induction s;intros.
 - split;intros;simpl in *. destruct H;try contradiction. inversion H. subst.
-  split;auto. exists 0. exists 0. now simpl. destruct_ctx.
+  split;auto. exists 0. exists 0. now simpl. d_ctx.
   rewrite firstn_nil in H0. rewrite skipn_nil in H0. subst. left; now simpl.
 - split;intros.
   * simpl in H. derive_plus_tac H. 
-    ** apply IHs in H. destruct_ctx. subst. split;auto. exists (S x). now simpl.
-    ** apply IHs in H. destruct_ctx. subst. split;auto. exists (S x).
+    ** apply IHs in H. d_ctx. subst. split;auto. exists (S x). now simpl.
+    ** apply IHs in H. d_ctx. subst. split;auto. exists (S x).
 
 Ltac derive_plus_tac H := rewrite derive_plus in H; simpl in H; apply in_app_or in H; destruct H.
 Theorem in_flatten_seq_o_derive : forall s e c0 c1 c_der0 c_der1, In (c_der0 _;_ c_der1) (flatten (((o c0) _;_ c1) // (e::s))) <-> 
@@ -793,8 +1476,8 @@ induction s;intros.
 - split;intros;simpl. destruct H;try contradiction. inversion H. subst.
   left.  split;autoC. exists 0. now simpl. destruct H;try contradiction. 
   inversion H. subst. right. split;autoC. exists 1. now simpl.
-  destruct H. destruct_ctx. subst. left. simpl. rewrite firstn_nil.
-  rewrite o_derive. auto.  destruct_ctx. destruct x. simpl in H0. subst. subst. right.
+  destruct H. d_ctx. subst. left. simpl. rewrite firstn_nil.
+  rewrite o_derive. auto.  d_ctx. destruct x. simpl in H0. subst. subst. right.
   rewrite o_idempotent. 
   auto. simpl in H0. subst. right. left. rewrite o_idempotent. auto.
 - split;intros.
@@ -802,35 +1485,35 @@ induction s;intros.
     derive_plus_tac H. rewrite Heql in H. rewrite o_derive in H.
     assert (HA : Failure = o Failure). { auto. } rewrite HA in H.
     apply IHs in H. destruct H.
-    ** destruct_ctx. subst. left.
+    ** d_ctx. subst. left.
  rewrite <- Heql in H. simpl in H. fold in H. derive_plus_tac H. 
     ** simpl in IHs. rewrite o_derive in H. assert (HA : Failure = o Failure). { auto. }
        rewrite HA in H. setoid_rewrite o_idempotent in IHs. 
        rewrite o_idempotent in H. apply IHs in H. destruct H.
-      *** destruct_ctx. subst. left. split;auto. destruct H. derive_plus_tac H.
+      *** d_ctx. subst. left. split;auto. destruct H. derive_plus_tac H.
       *** simpl in IHs. rewrite derive_plus in H. simpl in H. simpl in H.
 
 
 
  left.
-  destruct (o_or c0); intuition. now exists 0. left. symmetry. destruct_ctx.
+  destruct (o_or c0); intuition. now exists 0. left. symmetry. d_ctx.
   destruct (o_or c0). destruct H. subst. rewrite H1. rewrite skipn_nil. auto.
   destruct H. contradiction. destruct H. subst. rewrite skipn_nil. auto.
   destruct H. contradiction.
 - split;intros.
   * rewrite derive_plus in H. simpl in H. apply in_app_or in H. destruct H.
     ** rewrite o_derive in H. assert (HA: Failure = o Failure). auto.
-       rewrite HA in H. apply IHs in H. destruct_ctx. subst. split.
+       rewrite HA in H. apply IHs in H. d_ctx. subst. split.
       *** destruct H.
         **** subst. right. split. intro H3. discriminate. auto.
         **** destruct H. subst. right. split. intro H3. discriminate. auto.
       *** destruct H. subst. exists (S x). auto. exists (S x). auto.
-    ** apply IHs in H. destruct_ctx. subst. destruct H.
+    ** apply IHs in H. d_ctx. subst. destruct H.
       *** split. subst. rewrite o_idempotent. now left. split.
  
 
   subst. rewrite H1. left.
-  destruct H. subst.  inversion H. now left. destruct_ctx. contradiction.
+  destruct H. subst.  inversion H. now left. d_ctx. contradiction.
 
 Theorem in_flatten_seq_derive : forall s c0 c1 c_der0 c_der1, In (c_der0 _;_ c_der1) (flatten ((c0 _;_ c1) // s)) <-> 
 (c_der0 _;_ c_der1 = c0 // s _;_ c1) \/ ( s<> [] /\ (c_der0 = Success \/ c_der0 = Failure) /\ exists n, c_der1 = c1//(skipn n s)).
@@ -838,12 +1521,12 @@ Proof.
 intro. 
 induction s;intros;simpl.
 - split;intros. destruct H;try contradiction. inversion H. subst. now left.
-  destruct H. inversion H. now left. destruct_ctx. contradiction.
+  destruct H. inversion H. now left. d_ctx. contradiction.
 - split;intros.
   * rewrite derive_plus in H. simpl in H. apply in_app_or in H. destruct H.
     ** apply IHs in H. destruct H.
       *** now left.
-      *** destruct_ctx. destruct H0.
+      *** d_ctx. destruct H0.
         **** subst. right. split.  intro H2.  discriminate. split. now left. 
              exists (S x). now simpl.
         **** subst. right. split. intro H2. discriminate. split. now right.
@@ -855,7 +1538,7 @@ induction s;intros;simpl.
   exists 1. now simpl. split. destruct H. inversion H. subst.
   destruct (o_or c0). rewrite H0. right. now left. rewrite H0. right. right. auto.
   inversion H. inversion H. inversion H0. subst. exists 0. now simpl.
-  inversion H0. destruct_ctx. destruct H. destruct x.
+  inversion H0. d_ctx. destruct H. destruct x.
   * simpl in H0. subst. intuition. auto.
  subst. destruct H;subst. simpl. now right. susbt. 
  rewrite H.
@@ -868,13 +1551,13 @@ c_der = (c0//s _;_ c1) \/ (s <> [] /\ exists n, c_der = Success _;_ (c1 // (skip
 Proof.
 induction s;intros.
 - simpl. split;intros. destruct H. now left. contradiction. destruct H. now left.
-  destruct_ctx. destruct H. auto.
+  d_ctx. destruct H. auto.
 - split;intros.
   * simpl in H. rewrite derive_plus in H. simpl in H.
     apply in_app_or in H. destruct H.
     ** apply IHs in H. destruct H.
       *** left. now simpl.
-      *** right. split;auto. intro H3. discriminate. destruct_ctx.
+      *** right. split;auto. intro H3. discriminate. d_ctx.
           destruct H0.
         **** rewrite H0. exists (S x). simpl. now left.
         **** rewrite H0. exists (S x). simpl. now right.
@@ -893,7 +1576,7 @@ induction s;intros.
           right. split. intro. discriminate. rewrite <- H. exists 0.
           destruct (o_or c0);rewrite H0; auto || auto.
       *** rewrite flatten_seq_trace_derive in H. rewrite in_flat_map in H.
-          destruct_ctx.
+          d_ctx.
         **** inversion
 
 
@@ -908,7 +1591,7 @@ Inductive Flat_Seq_Derivative : Contract -> Contract -> Trace -> nat -> list Con
 | FSD_Single c0 c1 s : Flat_Seq_Derivative c0 c1 s 0 [c0//s _;_ c1]
 | FSD_Cons c0 c1 s n l (H: Flat_Seq_Derivative c0 c1 s n l) : Flat_Seq_Derivative c0 c1 s (S n) (c1//(firstn (S n) s)::l).
 
-Ltac in_forall HF HIn := rewrite Forall_forall in HF; apply HF in HIn;destruct_ctx;subst.
+Ltac in_forall HF HIn := rewrite Forall_forall in HF; apply HF in HIn;d_ctx;subst.
 
 Lemma flatten_seq_derive_FSD : forall c0 c1 c_der s l, Flat_Seq_Derivative c0 c1 s (length s) l -> 
  In c_der (flatten ((c0 _;_ c1) // s)) <-> ((exists c', c' =R= c_der /\ In c' l) \/ c_der =R= Failure).
@@ -924,7 +1607,7 @@ intros. remember (length s). induction H.
 
   * inversion H1. subst. rewrite H.  auto using in_eq. contradiction.
   * rewrite H in H1. simpl in H1. destruct H1;auto.
-    rewrite Forall_forall in H0. apply H0 in H1. destruct_ctx. subst.
+    rewrite Forall_forall in H0. apply H0 in H1. d_ctx. subst.
     ** now left. 
     rewrite Forall_forall in H1.
 
@@ -947,7 +1630,7 @@ induction l;intros.
 - simpl in H0. inversion H0.
   * rewrite derive_plus in H. simpl in H.
   destruct (flatten_non_empty ((c0 / a _;_ c1) // s)).
-  destruct_ctx. rewrite H0 in H. simpl in H. apply in_app_or in H.
+  d_ctx. rewrite H0 in H. simpl in H. apply in_app_or in H.
   destruct H.
   *
 
@@ -978,7 +1661,7 @@ induction c;intros.
 - exists [Success;Failure]. split;auto with dpDB. 
 - exists [Failure]. split;auto with dpDB.
 - exists [Event e;Success;Failure]. split;auto with dpDB.
-- destruct_ctx. exists (plus_prod x0 x). split;simpl; auto with dpDB.
+- d_ctx. exists (plus_prod x0 x). split;simpl; auto with dpDB.
   rewrite plus_prod_length. rewrite H2. now rewrite H0.
 -
   rewrite prod_length.
